RocqOfRust/revm/revm_interpreter/instructions/simulate/system/calldatasize.v
@@ -1,6 +1,7 @@
 Require Import simulate.RocqOfRust.
 Require Import core.slice.simulate.mod.
 Require Import revm.revm_interpreter.gas.simulate.constants.
+Require Import revm.revm_interpreter.interpreter_action.simulate.call_inputs.
 Require Import revm.revm_interpreter.instructions.links.system.calldatasize.
 Require Import revm.revm_interpreter.instructions.simulate.macros.
 Require Import revm.revm_interpreter.links.interpreter.
@@ -15,15 +16,14 @@ Definition calldatasize
     {IInterpreterTypes : InterpreterTypes.C WIRE_types}
     (interpreter : Interpreter.t WIRE WIRE_types) :
     Interpreter.t WIRE WIRE_types :=
-  gas_macro interpreter constants.BASE id (fun interpreter =>
   let input :=
     IInterpreterTypes.(InterpreterTypes.InputsTrait_for_Input).(InputTraits.input)
       .(RefStub.projection) interpreter.(Interpreter.input) in
-  let length : usize := Impl_Slice.len input in
+  let length : usize := call_inputs.CallInput.len input in
   push_macro interpreter
     (Impl_Uint.from length)
     id id
-  ).
+  .
 
 Lemma calldatasize_eq
     {WIRE H : Set} `{Link WIRE} `{Link H}
@@ -36,9 +36,13 @@ Lemma calldatasize_eq
     (host : H) :
   let ref_interpreter := make_ref 0 in
   let ref_host := make_ref (A := H) 1 in
+  let context := {|
+    instruction_context.InstructionContext.interpreter := ref_interpreter;
+    instruction_context.InstructionContext.host := ref_host;
+  |} in
     {{
       SimulateM.eval_f
-        (run_calldatasize run_InterpreterTypes_for_WIRE ref_interpreter ref_host)
+        (run_calldatasize run_InterpreterTypes_for_WIRE context)
         [interpreter; host]%stack 🌲
       (
         Output.Success tt,
@@ -47,13 +51,31 @@ Lemma calldatasize_eq
     }}.
 Proof.
   with_strategy transparent [run_calldatasize] unfold calldatasize, run_calldatasize; cbn.
-  gas_macro_eq idtac.
   s. {
     apply InterpreterTypesEq.
   }
   s. {
-    pose proof (Impl_Slice.len_eq (T := u8)) as H_apply.
-    s_apply H_apply.
+    apply call_inputs.CallInput.len_eq with
+      (self :=
+        IInterpreterTypes.(InterpreterTypes.InputsTrait_for_Input).(InputTraits.input)
+          .(RefStub.projection) interpreter.(Interpreter.input)).
+    cbn.
+    refine (@CanRead.Mutable
+      _ _
+      Pointer.Kind.Ref
+      [interpreter; host]%stack
+      (IInterpreterTypes.(InterpreterTypes.InputsTrait_for_Input).(InputTraits.input)
+        .(RefStub.projection) interpreter.(Interpreter.input))
+      _
+      (@Stack.CanAccess.Mutable
+        _ _
+        [interpreter; host]%stack
+        0
+        (Interpreter.t WIRE WIRE_types)
+        (@Stack.Nth.ConsZero (Interpreter.t WIRE WIRE_types) interpreter [host]%stack)
+        _ _ _ _)
+      _).
+    reflexivity.
   }
   s. {
     s_apply Impl_Uint.from_eq.
